src/Std/Data/DTreeMap/Internal/Model.lean
@@ -493,6 +493,14 @@ theorem maxKey?_eq_minKey?_reverse [Ord α] {l : Impl α β} :
     l.maxKey? = (letI : Ord α := .opposite inferInstance; (reverse l).minKey?) := by
   induction l using maxKey?.induct <;> simp_all only [minKey?, maxKey?, reverse]
 
+theorem some_maxKey_eq_maxKey? [Ord α] {l : Impl α β} {he} :
+    some (l.maxKey he) = l.maxKey? := by
+  induction l, he using maxKey.induct <;> simp_all [maxKey, maxKey?]
+
+theorem maxKey_eq_get_maxKey? [Ord α] {l : Impl α β} {he} :
+    l.maxKey he = l.maxKey?.get (by simp [← some_maxKey_eq_maxKey? (he := he)]) := by
+  simp [← some_maxKey_eq_maxKey? (he := he)]
+
 theorem balanceL_eq_balance {k : α} {v : β k} {l r : Impl α β} {hlb hrb hlr} :
     balanceL k v l r hlb hrb hlr = balance k v l r hlb hrb (Or.inl hlr.erase) := by
   rw [balanceL_eq_balanceLErase, balanceLErase_eq_balanceL!,
